Redesigning M typing rule a little

SkLean/Ast2.lean
@@ -171,12 +171,6 @@ inductive is_eval_once_weak : Expr → Expr → Prop
   | left         : is_eval_once_weak lhs lhs'
     → is_eval_once_weak SKM[(lhs rhs)] SKM[(lhs' rhs)]
 
-inductive beta_eq : SkExpr → SkExpr → Prop
-  | rfl                       : beta_eq e e
-  | eval                      : is_eval_once e₁ e₂ → beta_eq e₁ e₂
-  | left                      : beta_eq lhs lhs'   → beta_eq SKM[(lhs rhs)] SKM[(lhs' rhs)]
-  | trans                     : beta_eq e₁ e₂ → beta_eq e₂ e₃ → beta_eq e₁ e₃
-
 inductive valid_judgment : Expr → Expr → Prop
   | k n                       : valid_judgment SKM[K n] (.k (.mk n.succ))
   | s n                       : valid_judgment SKM[S n] (.s (.mk n.succ))
@@ -195,7 +189,7 @@ inductive valid_judgment : Expr → Expr → Prop
           rhs
         ))
       ))
-  | step_beta_eq e t₁ t₂           : valid_judgment e t₁ → is_eval_once t₁ t₂ → valid_judgment e t₂
+  | step_beta_eq e t₁ t₂           : valid_judgment e t₂ → is_eval_once t₁ t₂ → valid_judgment e t₁
 
 inductive valid_judgment_weak : Expr → Expr → Prop
   | k n                       : valid_judgment_weak SKM[K n] (.k (.mk n.succ))
@@ -218,10 +212,18 @@ inductive valid_judgment_weak : Expr → Expr → Prop
 
 end
 
+inductive beta_eq : SkExpr → SkExpr → Prop
+  | rfl                       : beta_eq e e
+  | eval                      : is_eval_once e₁ e₂ → beta_eq e₁ e₂
+  | left                      : beta_eq lhs lhs'   → beta_eq SKM[(lhs rhs)] SKM[(lhs' rhs)]
+  | trans                     : beta_eq e₁ e₂      → beta_eq e₂ e₃ → beta_eq e₁ e₃
+
 inductive is_normal_n : ℕ → Expr → Expr → Prop
   | stuck : (¬(∃ e', is_eval_once e e'))                 → is_normal_n 0 e e
   | one   : is_eval_once e e                             → is_normal_n 1 e e
   | succ  : is_eval_once e e' → is_normal_n n e' e_final → is_normal_n n.succ e e_final
+
+namespace is_normal_n
 
 lemma m_stuck : is_normal_n 0 SKM[M n] SKM[M n] := by
   apply is_normal_n.stuck
@@ -241,3 +243,4 @@ lemma s_stuck : is_normal_n 0 SKM[S n] SKM[S n] := by
   obtain ⟨e', h_eval⟩ := h
   cases h_eval
 
+end is_normal_n
