SkLean/Sn2.lean
@@ -16,7 +16,7 @@ lemma sn_call_s : sn SKM[((((S n) x) y) z)] → sn SKM[((x z) (y z))] := by
     | .hard h_step =>
       exact h_step SKM[((x z) (y z))] (by apply is_eval_once.s)
 
-lemma sn_m : sn SKM[(M n e)] → valid_judgment e t → sn t := by
+lemma sn_call_m : sn SKM[(M n e)] → valid_judgment e t → sn t := by
   intro h_sn h_t
   match h_sn with
     | .hard h_step =>
@@ -33,50 +33,47 @@ lemma sn_preserved : sn e → is_eval_once e e' → sn e' := by
       | .hard h_step =>
         exact h_step e' h_eval
 
-lemma sn_imp_n_steps_eval_normal (e : Expr) : sn e → ∃ n e', is_normal_n n e e' := by
-  intro h_sn
-  match h_eq : e with
-    | SKM[(M n₁)] =>
-      use 0
-      use SKM[(M n₁)]
-      apply m_stuck
-    | SKM[(K n)] =>
-      use 0
-      use SKM[(K n)]
-      apply k_stuck
-    | SKM[(S n)] =>
-      use 0
-      use SKM[(S n)]
-      apply s_stuck
-    | SKM[(((K n_k) x) y)] =>
-      match h_sn with
-        | .hard h =>
-          have h := h x (by apply is_eval_once.k)
-          have ⟨n, e_norm, h_norm_step⟩ := sn_imp_n_steps_eval_normal _ h
-          use n.succ
-          use e_norm
-          apply is_normal_n.succ
-          apply is_eval_once.k
-          exact h_norm_step
-    | SKM[((((S n) x) y) z)] =>
-      rw [← h_eq] at h_sn
-      induction h_sn
-      case hard e' h_step hh =>
-        have h_eval := is_eval_once.s x y z n
-        rw [h_eq] at h_step
-        rw [h_eq] at hh
-        have h_eval_sn := h_step _ h_eval
-        cases h_eval_sn
-        
+lemma sn_imp_n_steps_eval_normal (e : Expr) : valid_judgment e t → sn e → ∃ n e', is_normal_n n e e' := by
+  intro h_t h_sn
+  induction h_sn
+  case hard e' h_step h_eval' =>
+    match e' with
+      | SKM[M n] =>
+        use 0
+        use SKM[M n]
+        apply m_stuck
+      | SKM[K n] =>
+        use 0
+        use SKM[K n]
+        apply k_stuck
+      | SKM[S n] =>
+        use 0
+        use SKM[S n]
+        apply s_stuck
+      | SKM[(((K n) x) y)] =>
+        have h_x_sn := h_step x (by apply is_eval_once.k)
+        have ⟨n_norm, norm_x, h_norm_x⟩ := h_eval' x (by apply is_eval_once.k) (by sorry)
+        use n_norm.succ
+        use norm_x
+        apply is_normal_n.succ
+        apply is_eval_once.k
+        exact h_norm_x
+      | SKM[((((S n) x) y) z)] =>
+        have h_eval_sn := h_step SKM[((x z) (y z))] (by apply is_eval_once.s)
+        have ⟨n_norm, norm_eval, h_norm_eval⟩ := h_eval' SKM[((x z) (y z))] (by apply is_eval_once.s) sorry
+        use n_norm.succ
+        use norm_eval
+        apply is_normal_n.succ
+        apply is_eval_once.s
+        exact h_norm_eval
+      | SKM[(M n e)] =>
+        have h_eval_sn := h_step t (by apply is_eval_once.m)
+        have ⟨n_norm, norm_eval, h_norm_eval⟩ := h_eval' SKM[((x z) (y z))] (by apply is_eval_once.s) sorry
+        use n_norm.succ
+        use norm_eval
+        apply is_normal_n.succ
+        apply is_eval_once.s
+        exact h_norm_eval
         sorry
-    | SKM[((M n) e)] =>
-      
-      sorry
-    | SKM[(lhs rhs)] =>
-      rw [← h_eq] at h_sn
-      induction h_sn
-      case hard e' h_step hh =>
-        simp_all
-        
-        sorry
+      | SKM[(lhs rhs)] => sorry
 
