SkLean/Typing2.lean
@@ -1,0 +1,112 @@
+import SkLean.Ast2
+
+namespace valid_judgment_weak
+
+lemma eval_preserves_judgment_hard : ∀ e e' t, valid_judgment_weak e t → is_eval_once e e' → valid_judgment_weak e' t := by
+  intro e e' t h_t h_eval
+  cases h_t
+  case k n =>
+    cases h_eval
+  case s =>
+    cases h_eval
+  case m =>
+    cases h_eval
+  case call lhs rhs h_u h_t_lhs h_t_rhs  =>
+    match h₀ : h_eval with
+      | .k lhs' rhs' n =>
+        cases h_t_lhs
+      | .s x' y' z' n =>
+        cases h_t_lhs
+      | .left h_eval' =>
+        cases h_t_lhs
+      | .m e t n h_t =>
+        cases h_t_lhs
+
+lemma weakening : valid_judgment_weak e t → valid_judgment e t := by
+  intro h
+  cases h
+  case k =>
+    apply valid_judgment.k
+  case s =>
+    apply valid_judgment.s
+  case m =>
+    apply valid_judgment.m
+  case call lhs rhs h_u h_t_lhs h_t_rhs =>
+    apply valid_judgment.call
+    exact h_u
+    apply weakening at h_t_lhs
+    exact h_t_lhs
+    apply weakening at h_t_rhs
+    exact h_t_rhs
+
+end valid_judgment_weak
+
+inductive has_final_judgment : Expr → Expr → Prop
+  | trivial : valid_judgment_weak e t → has_final_judgment e t
+  | hard    : is_eval_once t t'       → has_final_judgment e t' → has_final_judgment e t
+
+namespace has_final_judgment
+
+lemma preserved : has_final_judgment e t → is_eval_once e e' → has_final_judgment e' t := by
+  intro h_t h_eval
+  induction h_t
+  case trivial e'' t' h =>
+    apply valid_judgment_weak.eval_preserves_judgment_hard at h
+    apply has_final_judgment.trivial
+    exact h h_eval
+  case hard t'' t''' e'' h_eval' h_final h_step =>
+    simp_all
+    apply has_final_judgment.hard
+    exact h_eval'
+    exact h_step
+
+lemma imp_valid_judgment : has_final_judgment e t → valid_judgment e t := by
+  intro h
+  induction h
+  case trivial h =>
+    apply valid_judgment_weak.weakening
+    exact h
+  case hard t'' t''' e' h_t_eq h_t h_t'' =>
+    apply valid_judgment.step_beta_eq
+    exact h_t''
+    exact h_t_eq
+
+lemma imp_exists_valid_judgment_weak : has_final_judgment e t → ∃ t, valid_judgment_weak e t := by
+  intro h
+  induction h
+  case trivial e' t' h =>
+    use t'
+  case hard t' t'' e' h_eval h_t' ih =>
+    exact ih
+
+end has_final_judgment
+
+namespace valid_judgment
+
+lemma imp_has_final_judgment : valid_judgment e t → has_final_judgment e t := by
+  intro h
+  cases h
+  case k =>
+    apply has_final_judgment.trivial
+    apply valid_judgment_weak.k
+  case s =>
+    apply has_final_judgment.trivial
+    apply valid_judgment_weak.s
+  case m =>
+    apply has_final_judgment.trivial
+    apply valid_judgment_weak.m
+  case call lhs rhs h_u h_t_lhs h_t_rhs =>
+    apply has_final_judgment.hard
+    
+    exact h_u
+    
+    sorry
+  case step_beta_eq t' h_t
+  sorry
+
+theorem preserved : valid_judgment e t → is_eval_once e e' → valid_judgment e' t := by
+  intro h_t h_eval
+  
+  sorry
+
+end valid_judgment
